verif/verif_putrecord.v
@@ -23,9 +23,148 @@ Require Import verif_splitnode.
 Lemma body_putEntry: semax_body Vprog Gprog f_putEntry putEntry_spec.
 Proof.
   start_function.
+  unfold cursor_rep. Intros anc_end. Intros idx_end.
+  destruct r as [root prel]. pose (r:=(root,prel)).
+  forward.                      (* t'44=cursor->level *)
+  forward_if.                   (* if t'44=-1 *)
+  (* split root case *)
+  - forward_call(false,true,true). (* t'1=createnewnode(false,true,true) *)
+    Intros vnewnode.
+    gather_SEP 1 2. replace_SEP 0 (cursor_rep c r pc).
+    { entailer!. unfold cursor_rep. Exists anc_end. Exists idx_end. unfold r. cancel.
+      change_compspecs CompSpecs. cancel. } clear anc_end. clear idx_end.
+    forward_if(PROP (vnewnode <> nullval) LOCAL (temp _currNode__1 vnewnode; temp _t'44 (Vint (Int.repr (Zlength c - 1))); temp _cursor pc; temp _newEntry pe; temp _key (key_repr oldk)) SEP (cursor_rep c r pc; btnode_rep (empty_node false true true vnewnode); relation_rep (root, prel); entry_rep e)).
+    + apply denote_tc_test_eq_split.
+      replace (vnewnode) with (getval (empty_node false true true vnewnode)). entailer!.
+      simpl. auto.
+      entailer!.
+    + forward.                  (* skip *)
+      entailer!.
+    + assert_PROP(False). unfold empty_node. entailer!. contradiction.
+    + unfold cursor_rep. Intros anc_end. Intros idx_end. unfold r.
+      forward.                  (* t'52=cursor->relation *)
+      unfold relation_rep. Intros.
+      forward.                  (* t'53=t'52->root *)
+      unfold empty_node.
+      rewrite unfold_btnode_rep. Intros ent_end.
+      forward.                  (* currnode1->ptr0=t'53 *)
+      forward.                  (* currnode1->numKeys=1 *)
+      admit.
+  - forward.                    (* skip *)
+    destruct c as [|[currnode entryidx] c'] eqn:HC.
+    { simpl in H0. exfalso. apply H3. rewrite Int.neg_repr. auto. }
+    forward_call(r,c,pc).       (* t'26=currnode(cursor) *)
+    { unfold r. unfold cursor_rep. Exists anc_end. Exists idx_end. cancel. change_compspecs CompSpecs.
+      cancel. rewrite HC. simpl. cancel. }
+    { rewrite HC. unfold r. split.
+      destruct H. right. auto. left. unfold ne_partial_cursor.
+      destruct H. split; auto. split; auto. simpl. omega. auto. }
+    rewrite HC. simpl.
+    assert(SUBNODE: subnode currnode root).
+    { destruct H. destruct H. apply complete_cursor_subnode in H. simpl in H. auto.
+      destruct H. apply partial_cursor_subnode in H. simpl in H. auto. }
+    assert(SUBREP: subnode currnode root) by auto.
+    apply subnode_rep in SUBREP.
+    destruct currnode as [ptr0 le isLeaf First Last x].
+    pose(currnode := btnode val ptr0 le isLeaf First Last x). simpl.
+    rewrite SUBREP. fold currnode.
+    rewrite unfold_btnode_rep with (n:=currnode) at 1. unfold currnode. Intros ent_end.
+    forward.                    (* t'27=t'26->isLeaf *)
+    { destruct isLeaf; entailer!. }
+    admit.
+Admitted.
+
+Lemma gotokey_complete: forall c r key,
+    complete_cursor c r ->
+    complete_cursor (goToKey c r key) r.
+Proof.
+Admitted.
+
+Lemma putentry_complete: forall c r e oldk newx d newc newr,
+    complete_cursor c r ->
+    putEntry val c r e oldk newx d = (newc, newr) ->
+    complete_cursor newc newr.
+Proof.
+Admitted.
+
+Lemma putentry_depth: forall c r e oldk newx d newc newr,
+    complete_cursor c r ->
+    correct_depth r ->
+    putEntry val c r e oldk newx d = (newc, newr) ->
+    correct_depth newr.
+Proof.
+Admitted.
+
+Lemma putentry_wf: forall c r e oldk newx d newc newr,
+    complete_cursor c r ->
+    root_wf (get_root r) ->
+    putEntry val c r e oldk newx d = (newc, newr) ->
+    root_wf (get_root newr).
+Proof.
+Admitted.
+
+Lemma putentry_integrity: forall c r e oldk newx d newc newr,
+    complete_cursor c r ->
+    root_integrity (get_root r) ->
+    putEntry val c r e oldk newx d = (newc, newr) ->
+    root_integrity (get_root newr).
+Proof.
+Admitted.
+
+Lemma putentry_numrec: forall c r e oldk newx d newc newr,
+    complete_cursor c r ->
+    Z.of_nat(get_numrec r) < Int.max_signed - 1 ->
+    putEntry val c r e oldk newx d = (newc, newr) ->
+    Z.of_nat(get_numrec newr) < Int.max_signed.
+Proof.
 Admitted.
 
 Lemma body_RL_PutRecord: semax_body Vprog Gprog f_RL_PutRecord RL_PutRecord_spec.
 Proof.
   start_function.
-Admitted.
+  forward_if(PROP (pc <> nullval)
+     LOCAL (lvar _newEntry (Tstruct _Entry noattr) v_newEntry; temp _cursor pc;
+     temp _key (key_repr key); temp _record (value_repr record))
+     SEP (data_at_ Tsh (Tstruct _Entry noattr) v_newEntry; relation_rep r; cursor_rep c r pc)).
+  - forward.                    (* skip *)
+    entailer!.
+  - assert_PROP(False). entailer!. contradiction.
+  - fold tentry.
+    forward.                    (* newentry.ptr.record=record *)
+    forward.                    (* newentry.key=key *)
+    forward_call(c,pc,r,key).   (* gotokey(cursor,key) *)
+    forward_call((goToKey c r key),pc,r,(keyval val key record (field_address tentry [UnionField _record; StructField _ptr] v_newEntry)), v_newEntry, key). (* putEntry(cursor,newEntry,key *)
+    + unfold entry_rep, value_rep, value_repr.
+      unfold_data_at 1%nat.
+      erewrite field_at_Tunion with (t:=tentry) (gfs:=[StructField _ptr]) (v1:=(inr(Vint(Int.repr(v_ record))))) (p:=v_newEntry).
+      2:reflexivity. 2:apply JMeq_refl.
+      simpl. unfold withspacer. rewrite if_true by omega.
+      rewrite field_at_data_at with (gfs:=[UnionField _record; StructField _ptr]).
+      simpl. cancel.
+    + split3; auto. left. apply gotokey_complete. auto.
+    + Intros newx.
+      destruct(putEntry val (goToKey c r key) r) as [newc newr] eqn:HPUTENTRY.
+      forward_call(newc,pc,newr). (* RL_MoveToNext(cursor) *)
+      * cancel.
+      * apply gotokey_complete with (key:=key) in H.
+        split3.
+        eapply putentry_complete. eauto. eauto.
+        eapply putentry_depth. eauto. eauto. eauto.
+        split3.
+        eapply putentry_wf. eauto. auto. eauto.
+        eapply putentry_integrity. eauto. auto. eauto.
+        eapply putentry_numrec. eauto. auto. eauto.
+      * forward.                (* return *)
+        Exists newx.
+        Exists((field_address tentry [UnionField _record; StructField _ptr] v_newEntry)).
+        entailer!. unfold RL_PutRecord.
+        rewrite HPUTENTRY.
+        cancel. fold tentry. unfold value_rep.
+        eapply derives_trans.
+        2:eapply data_at_data_at_ with (v:=(key_repr key, inr (value_repr record))).
+        unfold_data_at 2%nat.
+        erewrite field_at_Tunion with (t:=tentry) (gfs:=[StructField _ptr]) (v1:=(inr(Vint(Int.repr(v_ record))))) (p:=v_newEntry).
+        2: reflexivity. 2: apply JMeq_refl.
+        simpl. unfold withspacer. rewrite if_true by omega. cancel.
+        rewrite field_at_data_at. simpl. cancel.
+Qed.
