verif/verif_splitnode.v
@@ -15,8 +15,24 @@ Require Import btrees.
 Require Import btrees_sep.
 Require Import btrees_spec.
 Require Import verif_newnode.
+Require Import verif_findindex.
 
 Lemma body_splitnode: semax_body Vprog Gprog f_splitnode splitnode_spec.
 Proof.
   start_function.
+  destruct n as [ptr0 le isLeaf First Last nval].
+  pose(n:=btnode val ptr0 le isLeaf First Last nval).
+  destruct(entry_val_rep e) as [keyrepr coprepr] eqn:HEVR.
+  assert(exists k, keyrepr = key_repr k).
+  { destruct e; exists k; simpl; simpl in HEVR; inv HEVR; auto. }
+  destruct H1 as [k HK].
+  forward.                      (* t'8=entry->key *)
+  forward_call(n,k).            (* t'1=findrecordindex(node,t'8) *)
+  { fold n. cancel. }
+  { split; auto. unfold node_wf. fold n in H0. omega. }
+  forward.                      (* tgtIdx=t'1 *)
+  forward.                      (* j=0 *)
+  forward.                      (* inserted=0 *)
+  (* forward_loop *)
+  admit.
 Admitted.
